UBody.FWf.allEq

FreydSSA/Body/Fun/Basic.lean
@@ -4,25 +4,38 @@ variable {φ ν α} [Φ : InstSet φ (Ty α)]
   [Φc : CohInstSet φ (Ty α)]
   [DecidableEq ν] [DecidableEq α]
 
-inductive UBody.FWf : FCtx ν (Ty α) → UBody φ ν → FCtx ν (Ty α) → Type _
-  | nil {Γ Δ} : Γ.Wk Δ → FWf Γ nil Δ
-  | let1 (x) : e.FWf p Γ A → FWf (Γ.cons x A) t Δ → FWf Γ (let1 x e t) Δ
-  | let2 (x y)
-    : e.FWf p Γ (Ty.pair A B) → FWf ((Γ.cons x A).cons y B) t Δ → FWf Γ (let2 x y e t) Δ
+inductive UBody.FWf : Purity → FCtx ν (Ty α) → UBody φ ν → FCtx ν (Ty α) → Type _
+  | nil (p) : Γ.Wk Δ → FWf p Γ nil Δ
+  | let1 (x) : e.FWf p Γ A → FWf p (Γ.cons x A) t Δ
+    → FWf p Γ (let1 x e t) Δ
+  | let2 (x y) : e.FWf p Γ (Ty.pair A B) →
+    FWf p ((Γ.cons x A).cons y B) t Δ → FWf p Γ (let2 x y e t) Δ
 
 def UBody.FWf.wk_entry {Γ' Γ Δ : FCtx ν (Ty α)} {t : UBody φ ν} (w: Γ'.Wk Γ)
-  : FWf Γ t Δ → FWf Γ' t Δ
-  | nil w' => nil (w.comp w')
+  : FWf p Γ t Δ → FWf p Γ' t Δ
+  | nil _ w' => nil _ (w.comp w')
   | let1 x de dt => let1 x (de.wk w) (dt.wk_entry (w.cons x _))
   | let2 x y de dt => let2 x y (de.wk w) (dt.wk_entry ((w.cons x _).cons y _))
 
-def UBody.FWf.wk_exit {Γ Δ Δ' : FCtx ν (Ty α)} {t : UBody φ ν} (dt : FWf Γ t Δ) (w: Δ.Wk Δ')
-  : FWf Γ t Δ' := match dt with
-  | nil w' => nil (w'.comp w)
+def UBody.FWf.wk_exit {Γ Δ Δ' : FCtx ν (Ty α)} {t : UBody φ ν} (dt : FWf p Γ t Δ) (w: Δ.Wk Δ')
+  : FWf p Γ t Δ' := match dt with
+  | nil _ w' => nil _ (w'.comp w)
   | let1 x de dt => let1 x de (dt.wk_exit w)
   | let2 x y de dt => let2 x y de (dt.wk_exit w)
 
---TODO: allEq, cmpTrg lore
+theorem UBody.FWf.allEq {Γ Δ : FCtx ν (Ty α)} {t : UBody φ ν} (dt : FWf p Γ t Δ) (dt' : FWf p Γ t Δ)
+  : dt = dt' := by induction dt with
+  | nil => cases dt'; rfl
+  | let1 x de dt I => cases dt' with | let1 x de' dt' =>
+    cases de.tyEq de'
+    cases de.allEq de'
+    rw [I]
+  | let2 x y de dt I => cases dt' with | let2 x y de' dt' =>
+    cases de.tyEq de'
+    cases de.allEq de'
+    rw [I]
+
+--TODO: cmpTrg lore
 
 --TODO: FWf.comp
 
